\section{Feynman 图}


%%%%%%%%%%%%%%%%%%%%%%%%%%%%%%%%%%%%%%%%%%%%%%%%%%%%%%%%%%%%%%
\subsection{Yukawa 理论}

















补充推导：

(7.21)
\begin{equation}
    \begin{aligned}
     \langle 0|\mathrm{i}T_{1}^{(1)}|\mathbf{p}^+,\lambda ;\mathbf{q}^-,\lambda ^{\prime};\mathbf{k}\rangle &=-\mathrm{i}\kappa \int{\mathrm{d}^4x}\langle 0|\mathrm{N} [ \phi (x)\bar{\psi}(x)\psi (x) ] |\mathbf{p}^+,\lambda ;\mathbf{q}^-,\lambda ^{\prime};\mathbf{k}\rangle 
\\
\text{缩并}&=\wick{-\mathrm{i}\kappa \int{\mathrm{d}^4x}\langle 0|\mathrm{N} [ \c3{\phi}(x)\c2{\bar{\psi}}(x)\c1{\psi}(x) ] |\c1{\mathbf{p}}^+,\lambda ;\c2{\mathbf{q}}^-,\lambda ^{\prime};\c3{\mathbf{k}}\rangle } 
\\
\text{调整}&=\wick{-\mathrm{i}\kappa \int{\mathrm{d}^4x}\langle 0|\mathrm{N} [ \c3{\phi}(x)\c2{\bar{\psi}}_a(x)\c1{\psi}_a(x) ] |\c1{\mathbf{p}}^+,\lambda ;\c2{\mathbf{q}}^-,\lambda ^{\prime};\c3{\mathbf{k}}\rangle }
\\
&=-\mathrm{i}\kappa \int{\mathrm{d}^4x}\langle 0|\phi ^{(+)}(x)\bar{\psi}_{a}^{(+)}(x)\psi _{a}^{(+)}(x)|\mathbf{p}^+,\lambda ;\mathbf{q}^-,\lambda ^{\prime};\mathbf{k}\rangle 
\\
&=-\mathrm{i}\kappa \int{\mathrm{d}^4x}\langle 0|\mathrm{e}^{-\mathrm{i}k\cdot x}\bar{v}_a(\mathbf{q},\lambda ^{\prime})\mathrm{e}^{-\mathrm{i}q\cdot x}u_a(\mathbf{p},\lambda )\mathrm{e}^{-\mathrm{i}p\cdot x}|0\rangle 
\\
\text{忽略下标}a&=-\mathrm{i}\kappa \int{\mathrm{d}^4x}\bar{v}_a(\mathbf{q},\lambda ^{\prime})u_a(\mathbf{p},\lambda )\mathrm{e}^{-\mathrm{i}\left( p+q+k \right) \cdot x}\langle 0|0\rangle 
\\
&=-\mathrm{i}\kappa \int{\mathrm{d}^4x}\bar{v}(\mathbf{q},\lambda ^{\prime})u(\mathbf{p},\lambda )\mathrm{e}^{-\mathrm{i}\left( p+q+k \right) \cdot x}
\\
\text{带一横在前}&=-\mathrm{i}\kappa \bar{v}(\mathbf{q},\lambda ^{\prime})u(\mathbf{p},\lambda )\left( 2\pi \right) ^4\delta ^{(4)}(p+q+k)
    \end{aligned}
\end{equation}





(7.28)
\begin{equation}
    \begin{aligned}
       \langle \mathbf{p}^+,\lambda ;\mathbf{q}^-,\lambda ^{\prime};\mathbf{k}|\mathrm{i}T_{1}^{(1)}|0\rangle &=-\mathrm{i}\kappa \int{\mathrm{d}^4}x\langle \mathbf{p}^+,\lambda ;\mathbf{q}^-,\lambda ^{\prime};\mathbf{k}|\mathrm{N}[ \phi (x)\bar{\psi}(x)\psi (x) ] |0\rangle 
\\
\text{缩并}&=\wick{-\mathrm{i}\kappa \int{\mathrm{d}^4}x\langle \c3{\mathbf{p}}^+,\lambda ;\c2{\mathbf{q}}^-,\lambda ^{\prime};\c1{\mathbf{k}}|\mathrm{N}[ \c1{\phi}(x)\c3{\bar{\psi}}(x)\c2{\psi}(x) ] |0\rangle }
\\
\text{调整}&=\wick{{\color[RGB]{240, 0, 0} +}\mathrm{i}\kappa \int{\mathrm{d}^4}x\langle \c3{\mathbf{p}}^+,\lambda ;\c2{\mathbf{q}}^-,\lambda ^{\prime};\c1{\mathbf{k}}|\mathrm{N}[ \c1{\phi}(x)\c2{\psi}_a(x)\c3{\bar{\psi}}_a(x) ] |0\rangle }
\\
&=+\mathrm{i}\kappa \int{\mathrm{d}^4}x\langle \mathbf{p}^+,\lambda ;\mathbf{q}^-,\lambda ^{\prime};\mathbf{k}|\phi ^{(-)}(x)\psi _{a}^{(-)}(x)\bar{\psi}_{a}^{(-)}(x)|0\rangle 
\\
&=+\mathrm{i}\kappa \int{\mathrm{d}^4}x\langle 0|\mathrm{e}^{\mathrm{i}k\cdot x}v_a(\mathbf{q},\lambda ^{\prime})\mathrm{e}^{\mathrm{i}q\cdot x}\bar{u}_a(\mathbf{p},\lambda )\mathrm{e}^{\mathrm{i}p\cdot x}|0\rangle 
\\
&=+\mathrm{i}\kappa \int{\mathrm{d}^4}xv_a(\mathbf{q},\lambda ^{\prime})\bar{u}_a(\mathbf{p},\lambda )\mathrm{e}^{\mathrm{i}\left( p+q+k \right) \cdot x}\langle 0|0\rangle 
\\
\text{忽略下标，调整横在前}&=+\mathrm{i}\kappa \int{\mathrm{d}^4}x\bar{u}(\mathbf{p},\lambda )v(\mathbf{q},\lambda ^{\prime})\mathrm{e}^{\mathrm{i}\left( p+q+k \right) \cdot x}
\\
\delta \text{函数性质}&=+\mathrm{i}\kappa \bar{u}(\mathbf{p},\lambda )v(\mathbf{q},\lambda ^{\prime})\left( 2\pi \right) ^4\delta ^{(4)}(p+q+k)
    \end{aligned}
\end{equation}

(7.32)b
\begin{equation}
    \begin{aligned}
        \langle \mathbf{p}^+,\lambda ;\mathbf{q}^-,\lambda ^{\prime}|\mathrm{i}T_{1}^{(1)}|\mathbf{k}\rangle &=-\mathrm{i}\kappa \int{\mathrm{d}^4}x\langle \mathbf{p}^+,\lambda ;\mathbf{q}^-,\lambda ^{\prime}|\mathrm{N} [ \phi (x)\bar{\psi}(x)\psi (x) ] |\mathbf{k}\rangle 
\\
\text{缩并}&=\wick{-\mathrm{i}\kappa \int{\mathrm{d}^4}x\langle \c1{\mathbf{p}}^+,\lambda ;\c2{\mathbf{q}}^-,\lambda ^{\prime}|\mathrm{N} [\c3{\phi}(x)\c1{\bar{\psi}}(x)\c2{\psi}(x) ] |\c3{\mathbf{k}}\rangle }
\\
\text{调整}&=\wick{+\mathrm{i}\kappa \int{\mathrm{d}^4}x\langle \c2{\mathbf{p}}^+,\lambda ;\c1{\mathbf{q}}^-,\lambda ^{\prime}|\mathrm{N} [ \c1{\psi}_a(x)\c2{\bar{\psi}}_a(x)\c3{\phi}(x) ] |\c3{\mathbf{k}}\rangle }
\\
\text{去正规乘积}&=+\mathrm{i}\kappa \int{\mathrm{d}^4}x\langle \mathbf{p}^+,\lambda ;\mathbf{q}^-,\lambda ^{\prime}|\psi _{a}^{(-)}(x)\bar{\psi}_{a}^{(-)}(x)\phi ^{(+)}(x)|\mathbf{k}\rangle 
\\
&=+\mathrm{i}\kappa \int{\mathrm{d}^4}x\langle 0|v_a(\mathbf{q},\lambda ^{\prime})\mathrm{e}^{\mathrm{i}q\cdot x}\bar{u}_a(\mathbf{p},\lambda )\mathrm{e}^{\mathrm{i}p\cdot x}\mathrm{e}^{-\mathrm{i}k\cdot x}|0\rangle 
\\
&=+\mathrm{i}\kappa \int{\mathrm{d}^4}xv_a(\mathbf{q},\lambda ^{\prime})\bar{u}_a(\mathbf{p},\lambda )\mathrm{e}^{-\mathrm{i}\left( k-p-q \right) \cdot x}\langle 0|0\rangle 
\\
&=+\mathrm{i}\kappa \int{\mathrm{d}^4}x\bar{u}(\mathbf{p},\lambda )v(\mathbf{q},\lambda ^{\prime})\mathrm{e}^{-\mathrm{i}\left( k-p-q \right) \cdot x}
\\
\text{有一横在前面}&=+\mathrm{i}\kappa \bar{u}(\mathbf{p},\lambda )v(\mathbf{q},\lambda ^{\prime})\left( 2\pi \right) ^4\delta ^{(4)}(k-p-q)
    \end{aligned}
\end{equation}

(7.33)c
\begin{equation}
    \begin{aligned}
        \langle \mathbf{q}^+,\lambda ^{\prime};\mathbf{k}|\mathrm{i}T_{1}^{(1)}|\mathbf{p}^+,\lambda \rangle &=-\mathrm{i}\kappa \int{\mathrm{d}^4}x\langle \mathbf{q}^+,\lambda ^{\prime};\mathbf{k}|\mathrm{N} [ \phi (x)\bar{\psi}(x)\psi (x) ] |\mathbf{p}^+,\lambda \rangle 
\\
\text{缩并}&=\wick{-\mathrm{i}\kappa \int{\mathrm{d}^4}x\langle \c2{\mathbf{q}}^+,\lambda ^{\prime};\c1{\mathbf{k}}|\mathrm{N} [ \c1{\phi}(x)\c2{\bar{\psi}}(x)\c3{\psi}(x) ] |\c3{\mathbf{p}}^+,\lambda \rangle }
\\
\text{整理}&=\wick{-\mathrm{i}\kappa \int{\mathrm{d}^4}x\langle \c2{\mathbf{q}}^+,\lambda ^{\prime};\c1{\mathbf{k}}|\mathrm{N} [\c1{\phi}(x)\c2{\bar{\psi}}_a(x)\c3{\psi}_a(x) ] |\c3{\mathbf{p}}^+,\lambda \rangle }
\\
\text{去正规乘积}&=-\mathrm{i}\kappa \int{\mathrm{d}^4}x\langle \mathbf{q}^+,\lambda ^{\prime};\mathbf{k}|\phi ^{(-)}(x)\bar{\psi}_{a}^{(-)}(x)\psi _{a}^{(+)}(x)|\mathbf{p}^+,\lambda \rangle 
\\
&=-\mathrm{i}\kappa \int{\mathrm{d}^4}x\langle 0|\mathrm{e}^{\mathrm{i}k\cdot x}\bar{u}_a(\mathbf{q},\lambda ^{\prime})\mathrm{e}^{\mathrm{i}q\cdot x}u_a(\mathbf{p},\lambda )\mathrm{e}^{-\mathrm{i}p\cdot x}|0\rangle 
\\
&=-\mathrm{i}\kappa \int{\mathrm{d}^4}x\bar{u}_a(\mathbf{q},\lambda ^{\prime})u_a(\mathbf{p},\lambda )\mathrm{e}^{-\mathrm{i}\left( p-q-k \right) \cdot x}\langle 0|0\rangle 
\\
&=-\mathrm{i}\kappa \int{\mathrm{d}^4}x\bar{u}(\mathbf{q},\lambda ^{\prime})u(\mathbf{p},\lambda )\mathrm{e}^{-\mathrm{i}\left( p-q-k \right) \cdot x}
\\
&=-\mathrm{i}\kappa \bar{u}(\mathbf{q},\lambda ^{\prime})u(\mathbf{p},\lambda )\left( 2\pi \right) ^4\delta ^{(4)}(p-q-k)
    \end{aligned}
\end{equation}



(7.34)d
\begin{equation}
    \begin{aligned}
        \langle \mathbf{q}^-,\lambda ^{\prime};\mathbf{k}|\mathrm{i}T_{1}^{(1)}|\mathbf{p}^-,\lambda \rangle &=-\mathrm{i}\kappa \int{\mathrm{d}^4x}\langle \mathbf{q}^-,\lambda ^{\prime};\mathbf{k}|\mathrm{N} [ \phi (x)\bar{\psi}_a(x)\psi _a(x) ] |\mathbf{p}^-,\lambda \rangle 
\\
\text{缩并}&=\wick{-\mathrm{i}\kappa \int{\mathrm{d}^4}x\langle \c3{\mathbf{q}}^-,\lambda ^{\prime};\c1{\mathbf{k}}|\mathrm{N} [ \c1{\phi}(x)\c2{\bar{\psi}}(x)\c3{\psi}(x) ] |\c2{\mathbf{p}}^-,\lambda \rangle }
\\
\text{调整}&=\wick{+\mathrm{i}\kappa \int{\mathrm{d}^4}x\langle \c2{\mathbf{q}}^-,\lambda ^{\prime};\c1{\mathbf{k}}|\mathrm{N} [ \c1{\phi}(x)\c2{\bar{\psi}}_a(x)\c3{\psi}_a(x) ] |\c3{\mathbf{p}}^-,\lambda \rangle }
\\
&=+\mathrm{i}\kappa \int{\mathrm{d}^4}x\langle \mathbf{q}^-,\lambda ^{\prime};\mathbf{k}|\phi ^{(-)}(x)\psi _{a}^{(-)}(x)\bar{\psi}_{a}^{(+)}(x)|\mathbf{p}^-,\lambda \rangle 
\\
&=+\mathrm{i}\kappa \int{\mathrm{d}^4}x\langle 0|\mathrm{e}^{\mathrm{i}k\cdot x}v_a(\mathbf{q},\lambda ^{\prime})\mathrm{e}^{\mathrm{i}q\cdot x}\bar{v}_a(\mathbf{p},\lambda )\mathrm{e}^{-\mathrm{i}p\cdot x}|0\rangle 
\\
&=+\mathrm{i}\kappa \int{\mathrm{d}^4}xv_a(\mathbf{q},\lambda ^{\prime})\bar{v}_a(\mathbf{p},\lambda )\mathrm{e}^{-\mathrm{i}\left( p-q-k \right) \cdot x}\langle 0|0\rangle 
\\
&=+\mathrm{i}\kappa \int{\mathrm{d}^4}x\bar{v}(\mathbf{p},\lambda )v(\mathbf{q},\lambda ^{\prime})\mathrm{e}^{-\mathrm{i}\left( p-q-k \right) \cdot x}
\\
&=+\mathrm{i}\kappa \bar{v}(\mathbf{p},\lambda )v(\mathbf{q},\lambda ^{\prime})\left( 2\pi \right) ^4\delta ^{(4)}(p-q-k)
    \end{aligned}
\end{equation}

(7.35)f
\begin{equation}
    \begin{aligned}
        \langle \mathbf{k}|\mathrm{i}T_{1}^{(1)}|\mathbf{p}^+,\lambda ;\mathbf{q}^-,\lambda ^{\prime}\rangle &=-\mathrm{i}\kappa \int{\mathrm{d}^4}x\langle \mathbf{k}|\mathrm{N}[ \phi (x)\bar{\psi}(x)\psi (x) ] |\mathbf{p}^+,\lambda ;\mathbf{q}^-,\lambda ^{\prime}\rangle 
\\
\text{缩并}&=\wick{-\mathrm{i}\kappa \int{\mathrm{d}^4}x\langle \c1{\mathbf{k}}|\mathrm{N} [ \c1{\phi}(x)\c3{\bar{\psi}}(x)\c2{\psi}(x) ] |\c2{\mathbf{p}}^+,\lambda ;\c3{\mathbf{q}}^-,\lambda ^{\prime}\rangle }
\\
\text{调整}&=\wick{-\mathrm{i}\kappa \int{\mathrm{d}^4}x\langle \c1{\mathbf{k}}|\mathrm{N} [ \c1{\phi}(x)\c3{\bar{\psi}}_a(x)\c2{\psi}_a(x) ] |\c2{\mathbf{p}}^+,\lambda ;\c3{\mathbf{q}}^-,\lambda ^{\prime}\rangle }
\\
\text{去正规乘积}&=-\mathrm{i}\kappa \int{\mathrm{d}^4}x\langle \mathbf{k}|\phi ^{(-)}(x)\bar{\psi}_{a}^{(+)}(x)\psi _{a}^{(+)}(x)|\mathbf{p}^+,\lambda ;\mathbf{q}^-,\lambda ^{\prime}\rangle 
\\
&=-\mathrm{i}\kappa \int{\mathrm{d}^4}x\langle 0|\mathrm{e}^{\mathrm{i}k\cdot x}\bar{v}_a(\mathbf{q},\lambda ^{\prime})\mathrm{e}^{-\mathrm{i}q\cdot x}u_a(\mathbf{p},\lambda )\mathrm{e}^{-\mathrm{i}p\cdot x}|0\rangle 
\\
&=-\mathrm{i}\kappa \int{\mathrm{d}^4}x\bar{v}_a(\mathbf{q},\lambda ^{\prime})u_a(\mathbf{p},\lambda )\mathrm{e}^{-\mathrm{i}\left( p+q-k \right) \cdot x}\langle 0|0\rangle 
\\
&=-\mathrm{i}\kappa \int{\mathrm{d}^4}x\bar{v}(\mathbf{q},\lambda ^{\prime})u(\mathbf{p},\lambda )\mathrm{e}^{-\mathrm{i}\left( p+q-k \right) \cdot x}
\\
\delta \text{函数性质}&=-\mathrm{i}\kappa \bar{v}(\mathbf{q},\lambda ^{\prime})u(\mathbf{p},\lambda )\left( 2\pi \right) ^4\delta ^{(4)}(p+q-k)
    \end{aligned}
\end{equation}


(7.36)g
\begin{equation}
    \begin{aligned}
        \langle \mathbf{q}^+,\lambda ^{\prime}|\mathrm{i}T_{1}^{(1)}|\mathbf{p}^+,\lambda ;\mathbf{k}\rangle &=-\mathrm{i}\kappa \int{\mathrm{d}^4}x\langle \mathbf{q}^+,\lambda ^{\prime}|\mathrm{N}[ \phi (x)\bar{\psi}(x)\psi (x) ] |\mathbf{p}^+,\lambda ;\mathbf{k}\rangle 
\\
\text{缩并}&=\wick{-\mathrm{i}\kappa \int{\mathrm{d}^4}x\langle \c1{\mathbf{q}}^+,\lambda ^{\prime}|\mathrm{N}[ \c3{\phi}(x)\c1{\bar{\psi}}(x)\c2{\psi}(x) ] |\c2{\mathbf{p}}^+,\lambda ;\c3{\mathbf{k}}\rangle }
\\
\text{调整}&=\wick{-\mathrm{i}\kappa \int{\mathrm{d}^4}x\langle \c1{\mathbf{q}}^+,\lambda ^{\prime}|\mathrm{N}[ \c1{\bar{\psi}}_a(x)\c3{\phi}(x)\c2{\psi}_a(x) ] |\c2{\mathbf{p}}^+,\lambda ;\c3{\mathbf{k}}\rangle }
\\
\text{去正规乘积}&=-\mathrm{i}\kappa \int{\mathrm{d}^4}x\langle \mathbf{q}^+,\lambda ^{\prime}|\bar{\psi}_{a}^{(-)}(x)\phi ^{(+)}(x)\psi _{a}^{(+)}(x)|\mathbf{p}^+,\lambda ;\mathbf{k}\rangle 
\\
&=-\mathrm{i}\kappa \int{\mathrm{d}^4}x\langle 0|\bar{u}_a(\mathbf{q},\lambda ^{\prime})\mathrm{e}^{\mathrm{i}q\cdot x}\mathrm{e}^{-\mathrm{i}k\cdot x}u_a(\mathbf{p},\lambda )\mathrm{e}^{-\mathrm{i}p\cdot x}|0\rangle 
\\
&=-\mathrm{i}\kappa \int{\mathrm{d}^4}x\bar{u}_a(\mathbf{q},\lambda ^{\prime})u_a(\mathbf{p},\lambda )\mathrm{e}^{-\mathrm{i}\left( p+k-q \right) \cdot x}\langle 0|0\rangle 
\\
&=-\mathrm{i}\kappa \int{\mathrm{d}^4}x\bar{u}(\mathbf{q},\lambda ^{\prime})u(\mathbf{p},\lambda )\mathrm{e}^{-\mathrm{i}\left( p+k-q \right) \cdot x}
\\
\text{函数性质}&=-\mathrm{i}\kappa \bar{u}(\mathbf{q},\lambda ^{\prime})u(\mathbf{p},\lambda )\left( 2\pi \right) ^4\delta ^{(4)}(p+k-q)
    \end{aligned}
\end{equation}


(7.37)h
\begin{equation}
    \begin{aligned}
        \langle \mathbf{q}^-,\lambda ^{\prime}|\mathrm{i}T_{1}^{(1)}|\mathbf{p}^-,\lambda ;\mathbf{k}\rangle &=-\mathrm{i}\kappa \int{\mathrm{d}^4}x\langle \mathbf{q}^-,\lambda ^{\prime}|\mathrm{N}[ \phi (x)\bar{\psi}(x)\psi (x) ] |\mathbf{p}^-,\lambda ;\mathbf{k}\rangle 
\\
\text{缩并}&=\wick{-\mathrm{i}\kappa \int{\mathrm{d}^4}x\langle \c1{\mathbf{q}}^-,\lambda ^{\prime}|\mathrm{N}[ \c2{\phi}(x)\c3{\bar{\psi}}(x)\c1{\psi}(x) ] |\c3{\mathbf{p}}^-,\lambda ;\c2{\mathbf{k}}\rangle }
\\
\text{调整}&=\wick{+\mathrm{i}\kappa \int{\mathrm{d}^4}x\langle \c1{\mathbf{q}}^-,\lambda ^{\prime}|\mathrm{N} [ \c1{\psi}_a(x)\c3{\phi}(x)\c2{\bar{\psi}}_a(x) ] |\c2{\mathbf{p}}^-,\lambda ;\c3{\mathbf{k}}\rangle }
\\
\text{正负能解}&=+\mathrm{i}\kappa \int{\mathrm{d}^4}x\langle \mathbf{q}^-,\lambda ^{\prime}|\psi _{a}^{(-)}(x)\phi (x)\bar{\psi}_{a}^{(+)}(x)|\mathbf{p}^-,\lambda ;\mathbf{k}\rangle 
\\
&=+\mathrm{i}\kappa \int{\mathrm{d}^4}x\langle 0|v_a(\mathbf{q},\lambda ^{\prime})\mathrm{e}^{\mathrm{i}q\cdot x}\mathrm{e}^{-\mathrm{i}k\cdot x}\bar{v}_a(\mathbf{p},\lambda )\mathrm{e}^{-\mathrm{i}p\cdot x}|0\rangle 
\\
&=+\mathrm{i}\kappa \int{\mathrm{d}^4}x\bar{v}_a(\mathbf{p},\lambda )v_a(\mathbf{q},\lambda ^{\prime})\mathrm{e}^{-\mathrm{i}\left( p+k-q \right) \cdot x}\langle 0|0\rangle 
\\
\text{横在前}&=+\mathrm{i}\kappa \int{\mathrm{d}^4}x\bar{v}(\mathbf{p},\lambda )v(\mathbf{q},\lambda ^{\prime})\mathrm{e}^{-\mathrm{i}\left( p+k-q \right) \cdot x}
\\
\text{函数性质}&=+\mathrm{i}\kappa \bar{v}(\mathbf{p},\lambda )v(\mathbf{q},\lambda ^{\prime})\left( 2\pi \right) ^4\delta ^{(4)}(p+k-q)
    \end{aligned}
\end{equation}


\newpage




\newpage
(7.58)无缩并
\begin{equation}
    \mathrm{i}T_{1}^{(2)}=\frac{\left( -\mathrm{i}\kappa \right) ^2}{2!}\int{\mathrm{d}^4x\mathrm{d}^4y\mathrm{N[}\phi (x)\bar{\psi}(x)\psi (x)\phi (y)\bar{\psi}(y)\psi (y)]}
\end{equation}

一次
\begin{equation}
    \begin{aligned}
        \mathrm{i}T_{2}^{(2)}&=\wick{ \frac{\left( -\mathrm{i}\kappa \right) ^2}{2!}\int{\mathrm{d}^4x\mathrm{d}^4y\mathrm{N} [ \c{\phi}(x)\bar{\psi}(x)\psi(x)\c{\phi}(y)\bar{\psi}(y)\psi (y)]} }
\\
\mathrm{i}T_{3}^{(2)}&=\frac{\left( -\mathrm{i}\kappa \right) ^2}{2!}\int{\mathrm{d}^4x\mathrm{d}^4y\mathrm{N} [ \phi (x)\bar{\psi}(x)\psi (x)\phi (y)\bar{\psi}(y)\psi (y)]}
\\
\mathrm{i}T_{4}^{(2)}&=\frac{\left( -\mathrm{i}\kappa \right) ^2}{2!}\int{\mathrm{d}^4x\mathrm{d}^4y\mathrm{N} [ \phi (x)\bar{\psi}(x)\psi (x)\phi (y)\bar{\psi}(y)\psi (y)]}
\\
\mathrm{i}T_{5}^{(2)}&=\frac{\left( -\mathrm{i}\kappa \right) ^2}{2!}\int{\mathrm{d}^4x\mathrm{d}^4y\mathrm{N} [ \phi (x)\bar{\psi}(x)\psi (x)\phi (y)\bar{\psi}(y)\psi (y)]}
\\
\mathrm{i}T_{6}^{(2)}&=\frac{\left( -\mathrm{i}\kappa \right) ^2}{2!}\int{\mathrm{d}^4x\mathrm{d}^4y\mathrm{N} [ \phi (x)\bar{\psi}(x)\psi (x)\phi (y)\bar{\psi}(y)\psi (y)]}
    \end{aligned}
\end{equation}

二次缩并





三次缩并




、



























