\section{}



\subsection{}

\subsection{推导：}
记得利用AI修改括号的形式

1.计算
\begin{equation}
    \begin{aligned}
        \bar{u}\left( \mathbf{p},\lambda \right) &=u^{\dagger}\left( \mathbf{p},\lambda \right) \gamma ^0
\\
&=\left( \begin{matrix}
	\omega _{-\lambda}\left( \mathbf{p} \right) \xi _{\lambda}^{\dagger}\left( \mathbf{p} \right)&		\omega _{\lambda}\left( \mathbf{p} \right) \xi _{\lambda}^{\dagger}\left( \mathbf{p} \right)\\
\end{matrix} \right) \left( \begin{matrix}
	&		1\\
	1&		\\
\end{matrix} \right) 
\\
&=\left( \begin{matrix}
	\omega _{\lambda}\left( \mathbf{p} \right) \xi _{\lambda}^{\dagger}\left( \mathbf{p} \right)&		\omega _{-\lambda}\left( \mathbf{p} \right) \xi _{\lambda}^{\dagger}\left( \mathbf{p} \right)\\
\end{matrix} \right) 
    \end{aligned}
\end{equation}
且
\begin{equation}
    \begin{aligned}
        \bar{v}\left( \mathbf{p},\lambda \right) &=v^{\dagger}\left( \mathbf{p},\lambda \right) \gamma ^0
\\
&=\left( \begin{matrix}
	\lambda \omega _{\lambda}\left( \mathbf{p} \right) \xi _{-\lambda}^{\dagger}\left( \mathbf{p} \right)&		-\lambda \omega _{-\lambda}\left( \mathbf{p} \right) \xi _{-\lambda}^{\dagger}\left( \mathbf{p} \right)\\
\end{matrix} \right) \left( \begin{matrix}
	&		1\\
	1&		\\
\end{matrix} \right) 
\\
&=\left( \begin{matrix}
	-\lambda \omega _{-\lambda}\left( \mathbf{p} \right) \xi _{-\lambda}^{\dagger}\left( \mathbf{p} \right)&		\lambda \omega _{\lambda}\left( \mathbf{p} \right) \xi _{-\lambda}^{\dagger}\left( \mathbf{p} \right)\\
\end{matrix} \right) 
    \end{aligned}
\end{equation}
2.计算
\begin{equation}
    \begin{aligned}
        \bar{u}\left( \mathbf{p},\lambda \right) u\left( \mathbf{p},\lambda \prime \right) &=\left( \begin{matrix}
	\omega _{\lambda}\left( \mathbf{p} \right) \xi _{\lambda}^{\dagger}\left( \mathbf{p} \right)&		\omega _{-\lambda}\left( \mathbf{p} \right) \xi _{\lambda}^{\dagger}\left( \mathbf{p} \right)\\
\end{matrix} \right) \left( \begin{array}{c}
	\omega _{-\lambda \prime}\left( \mathbf{p} \right) \xi _{\lambda \prime}\left( \mathbf{p} \right)\\
	\omega _{\lambda \prime}\left( \mathbf{p} \right) \xi _{\lambda \prime}\left( \mathbf{p} \right)\\
\end{array} \right) 
\\
&=\omega _{\lambda}\left( \mathbf{p} \right) \xi _{\lambda}^{\dagger}\left( \mathbf{p} \right) \omega _{-\lambda \prime}\left( \mathbf{p} \right) \xi _{\lambda \prime}\left( \mathbf{p} \right) +\omega _{-\lambda}\left( \mathbf{p} \right) \xi _{\lambda}^{\dagger}\left( \mathbf{p} \right) \omega _{\lambda \prime}\left( \mathbf{p} \right) \xi _{\lambda \prime}\left( \mathbf{p} \right) 
\\
&=\omega _{\lambda}\left( \mathbf{p} \right) \omega _{-\lambda \prime}\left( \mathbf{p} \right) \xi _{\lambda}^{\dagger}\left( \mathbf{p} \right) \xi _{\lambda \prime}\left( \mathbf{p} \right) +\omega _{-\lambda}\left( \mathbf{p} \right) \omega _{\lambda \prime}\left( \mathbf{p} \right) \xi _{\lambda}^{\dagger}\left( \mathbf{p} \right) \xi _{\lambda \prime}\left( \mathbf{p} \right) 
\\
&=\left[ \omega _{\lambda}\left( \mathbf{p} \right) \omega _{-\lambda \prime}\left( \mathbf{p} \right) +\omega _{-\lambda}\left( \mathbf{p} \right) \omega _{\lambda \prime}\left( \mathbf{p} \right) \right] \xi _{\lambda}^{\dagger}\left( \mathbf{p} \right) \xi _{\lambda \prime}\left( \mathbf{p} \right) 
\\
&=\left[ \omega _{\lambda}\left( \mathbf{p} \right) \omega _{-\lambda \prime}\left( \mathbf{p} \right) +\omega _{-\lambda}\left( \mathbf{p} \right) \omega _{\lambda \prime}\left( \mathbf{p} \right) \right] \delta _{\lambda \lambda \prime}
\\
&=\left[ \omega _{\lambda}\left( \mathbf{p} \right) \omega _{-\lambda}\left( \mathbf{p} \right) +\omega _{-\lambda}\left( \mathbf{p} \right) \omega _{\lambda}\left( \mathbf{p} \right) \right] \delta _{\lambda \lambda \prime}
\\
&=\left[ \omega _{\lambda}\left( \mathbf{p} \right) \omega _{-\lambda}\left( \mathbf{p} \right) +\omega _{\lambda}\left( \mathbf{p} \right) \omega _{-\lambda}\left( \mathbf{p} \right) \right] \delta _{\lambda \lambda \prime}
\\
&=2\omega _{\lambda}\left( \mathbf{p} \right) \omega _{-\lambda}\left( \mathbf{p} \right) \delta _{\lambda \lambda \prime}
\\
&=2m\delta _{\lambda \lambda \prime}
    \end{aligned}
\end{equation}
且
\begin{equation}
    \begin{aligned}
        \bar{v}\left( \mathbf{p},\lambda \right) v\left( \mathbf{p},\lambda ^{\prime} \right) &=\left( \begin{matrix}
	-\lambda \omega _{-\lambda}\left( \mathbf{p} \right) \xi _{-\lambda}^{\dagger}\left( \mathbf{p} \right)&		\lambda \omega _{\lambda}\left( \mathbf{p} \right) \xi _{-\lambda}^{\dagger}\left( \mathbf{p} \right)\\
\end{matrix} \right) \left( \begin{array}{c}
	\lambda \prime \omega _{\lambda \prime}\left( \mathbf{p} \right) \xi _{-\lambda \prime}\left( \mathbf{p} \right)\\
	-\lambda \prime \omega _{-\lambda \prime}\left( \mathbf{p} \right) \xi _{-\lambda \prime}\left( \mathbf{p} \right)\\
\end{array} \right) 
\\
&=-\lambda \omega _{-\lambda}\left( \mathbf{p} \right) \xi _{-\lambda}^{\dagger}\left( \mathbf{p} \right) \cdot \lambda \prime \omega _{\lambda \prime}\left( \mathbf{p} \right) \xi _{-\lambda \prime}\left( \mathbf{p} \right) -\lambda \omega _{\lambda}\left( \mathbf{p} \right) \xi _{-\lambda}^{\dagger}\left( \mathbf{p} \right) \cdot \lambda \prime \omega _{-\lambda \prime}\left( \mathbf{p} \right) \xi _{-\lambda \prime}\left( \mathbf{p} \right) 
\\
&=-\lambda \lambda \prime \omega _{-\lambda}\left( \mathbf{p} \right) \omega _{\lambda \prime}\left( \mathbf{p} \right) \cdot \xi _{-\lambda}^{\dagger}\left( \mathbf{p} \right) \xi _{-\lambda \prime}\left( \mathbf{p} \right) -\lambda \lambda \prime \omega _{\lambda}\left( \mathbf{p} \right) \omega _{-\lambda \prime}\left( \mathbf{p} \right) \cdot \xi _{-\lambda}^{\dagger}\left( \mathbf{p} \right) \xi _{-\lambda \prime}\left( \mathbf{p} \right) 
\\
&=-\lambda \lambda \prime \left[ \omega _{-\lambda}\left( \mathbf{p} \right) \omega _{\lambda \prime}\left( \mathbf{p} \right) +\omega _{\lambda}\left( \mathbf{p} \right) \omega _{-\lambda \prime}\left( \mathbf{p} \right) \right] \xi _{-\lambda}^{\dagger}\left( \mathbf{p} \right) \xi _{-\lambda \prime}\left( \mathbf{p} \right) 
\\
&=-\lambda \lambda \prime \left[ \omega _{-\lambda}\left( \mathbf{p} \right) \omega _{\lambda \prime}\left( \mathbf{p} \right) +\omega _{\lambda}\left( \mathbf{p} \right) \omega _{-\lambda \prime}\left( \mathbf{p} \right) \right] \delta _{\lambda \lambda \prime}
\\
&=-\lambda ^2\left[ \omega _{-\lambda}\left( \mathbf{p} \right) \omega _{\lambda}\left( \mathbf{p} \right) +\omega _{\lambda}\left( \mathbf{p} \right) \omega _{-\lambda}\left( \mathbf{p} \right) \right] \delta _{\lambda \lambda \prime}
\\
&=-\lambda ^2\left[ \omega _{\lambda}\left( \mathbf{p} \right) \omega _{-\lambda}\left( \mathbf{p} \right) +\omega _{\lambda}\left( \mathbf{p} \right) \omega _{-\lambda}\left( \mathbf{p} \right) \right] \delta _{\lambda \lambda \prime}
\\
&=-2\lambda ^2\omega _{\lambda}\left( \mathbf{p} \right) \omega _{-\lambda}\left( \mathbf{p} \right) \delta _{\lambda \lambda \prime}
\\
&=-2m\delta _{\lambda \lambda ^{\prime}}
    \end{aligned}
\end{equation}
且
\begin{equation}
    \begin{aligned}
        \begin{aligned}
            \bar{u}\left( \mathbf{p},\lambda \right) v\left( \mathbf{p},\lambda ^{\prime} \right) &=\left( \begin{matrix}
	\omega _{\lambda}\left( \mathbf{p} \right) \xi _{\lambda}^{\dagger}\left( \mathbf{p} \right)&		\omega _{-\lambda}\left( \mathbf{p} \right) \xi _{\lambda}^{\dagger}\left( \mathbf{p} \right)\\
\end{matrix} \right) \left( \begin{array}{c}
	\lambda \prime \omega _{\lambda \prime}\left( \mathbf{p} \right) \xi _{-\lambda \prime}\left( \mathbf{p} \right)\\
	-\lambda \prime \omega _{-\lambda \prime}\left( \mathbf{p} \right) \xi _{-\lambda \prime}\left( \mathbf{p} \right)\\
\end{array} \right) 
\\
&=\omega _{\lambda}\left( \mathbf{p} \right) \xi _{\lambda}^{\dagger}\left( \mathbf{p} \right) \cdot \lambda \prime \omega _{\lambda \prime}\left( \mathbf{p} \right) \xi _{-\lambda \prime}\left( \mathbf{p} \right) -\omega _{-\lambda}\left( \mathbf{p} \right) \xi _{\lambda}^{\dagger}\left( \mathbf{p} \right) \cdot \lambda \prime \omega _{-\lambda \prime}\left( \mathbf{p} \right) \xi _{-\lambda \prime}\left( \mathbf{p} \right) 
\\
&=\lambda \prime \omega _{\lambda}\left( \mathbf{p} \right) \omega _{\lambda \prime}\left( \mathbf{p} \right) \cdot \xi _{\lambda}^{\dagger}\left( \mathbf{p} \right) \xi _{-\lambda \prime}\left( \mathbf{p} \right) -\lambda \prime \omega _{-\lambda}\left( \mathbf{p} \right) \omega _{-\lambda \prime}\left( \mathbf{p} \right) \cdot \xi _{\lambda}^{\dagger}\left( \mathbf{p} \right) \xi _{-\lambda \prime}\left( \mathbf{p} \right) 
\\
&=\lambda \prime \left[ \omega _{\lambda}\left( \mathbf{p} \right) \omega _{\lambda \prime}\left( \mathbf{p} \right) -\omega _{-\lambda}\left( \mathbf{p} \right) \omega _{-\lambda \prime}\left( \mathbf{p} \right) \right] \xi _{\lambda}^{\dagger}\left( \mathbf{p} \right) \xi _{-\lambda \prime}\left( \mathbf{p} \right) 
\\
&=\lambda ^{\prime}\left[ \omega _{\lambda}\left( \mathbf{p} \right) \omega _{\lambda ^{\prime}}\left( \mathbf{p} \right) -\omega _{-\lambda}\left( \mathbf{p} \right) \omega _{-\lambda ^{\prime}}\left( \mathbf{p} \right) \right] \delta _{\lambda ,-\lambda ^{\prime}}
\\
&=-\lambda \left[ \omega _{\lambda}\left( \mathbf{p} \right) \omega _{-\lambda}\left( \mathbf{p} \right) -\omega _{-\lambda}\left( \mathbf{p} \right) \omega _{\lambda}\left( \mathbf{p} \right) \right] \delta _{\lambda ,-\lambda ^{\prime}}
\\
&=-\lambda \left[ \omega _{\lambda}\left( \mathbf{p} \right) \omega _{-\lambda}\left( \mathbf{p} \right) -\omega _{\lambda}\left( \mathbf{p} \right) \omega _{-\lambda}\left( \mathbf{p} \right) \right] \delta _{\lambda ,-\lambda ^{\prime}}
\\
&=0
        \end{aligned}
    \end{aligned}
\end{equation}
且
\begin{equation}
    \begin{aligned}
        \bar{v}\left( \mathbf{p},\lambda \right) u\left( \mathbf{p},\lambda ^{\prime} \right) &=\left( \begin{matrix}
	-\lambda \omega _{-\lambda}\left( \mathbf{p} \right) \xi _{-\lambda}^{\dagger}\left( \mathbf{p} \right)&		\lambda \omega _{\lambda}\left( \mathbf{p} \right) \xi _{-\lambda}^{\dagger}\left( \mathbf{p} \right)\\
\end{matrix} \right) \left( \begin{array}{c}
	\omega _{-\lambda \prime}\left( \mathbf{p} \right) \xi _{\lambda \prime}\left( \mathbf{p} \right)\\
	\omega _{\lambda \prime}\left( \mathbf{p} \right) \xi _{\lambda \prime}\left( \mathbf{p} \right)\\
\end{array} \right) 
\\
&=-\lambda \omega _{-\lambda}\left( \mathbf{p} \right) \xi _{-\lambda}^{\dagger}\left( \mathbf{p} \right) \cdot \omega _{-\lambda \prime}\left( \mathbf{p} \right) \xi _{\lambda \prime}\left( \mathbf{p} \right) +\lambda \omega _{\lambda}\left( \mathbf{p} \right) \xi _{-\lambda}^{\dagger}\left( \mathbf{p} \right) \cdot \omega _{\lambda \prime}\left( \mathbf{p} \right) \xi _{\lambda \prime}\left( \mathbf{p} \right) 
\\
&=-\lambda \omega _{-\lambda}\left( \mathbf{p} \right) \omega _{-\lambda \prime}\left( \mathbf{p} \right) \cdot \xi _{-\lambda}^{\dagger}\left( \mathbf{p} \right) \xi _{\lambda \prime}\left( \mathbf{p} \right) +\lambda \omega _{\lambda}\left( \mathbf{p} \right) \omega _{\lambda \prime}\left( \mathbf{p} \right) \cdot \xi _{-\lambda}^{\dagger}\left( \mathbf{p} \right) \xi _{\lambda \prime}\left( \mathbf{p} \right) 
\\
&=\lambda \left[ -\omega _{-\lambda}\left( \mathbf{p} \right) \omega _{-\lambda ^{\prime}}\left( \mathbf{p} \right) +\omega _{\lambda}\left( \mathbf{p} \right) \omega _{\lambda ^{\prime}}\left( \mathbf{p} \right) \right] \xi _{-\lambda}^{\dagger}\left( \mathbf{p} \right) \xi _{\lambda ^{\prime}}\left( \mathbf{p} \right) 
\\
&=\lambda \left[ -\omega _{-\lambda}\left( \mathbf{p} \right) \omega _{-\lambda ^{\prime}}\left( \mathbf{p} \right) +\omega _{\lambda}\left( \mathbf{p} \right) \omega _{\lambda ^{\prime}}\left( \mathbf{p} \right) \right] \delta _{-\lambda ,\lambda ^{\prime}}
\\
&=\lambda \left[ -\omega _{-\lambda}\left( \mathbf{p} \right) \omega _{\lambda}\left( \mathbf{p} \right) +\omega _{\lambda}\left( \mathbf{p} \right) \omega _{-\lambda}\left( \mathbf{p} \right) \right] \delta _{-\lambda ,\lambda ^{\prime}}
\\
&=\lambda \left[ -\omega _{\lambda}\left( \mathbf{p} \right) \omega _{-\lambda}\left( \mathbf{p} \right) +\omega _{\lambda}\left( \mathbf{p} \right) \omega _{-\lambda}\left( \mathbf{p} \right) \right] \delta _{-\lambda ,\lambda ^{\prime}}
\\
&=0
    \end{aligned}
\end{equation}
汇总结论




\subsection{推导：螺旋度求和关系=自旋求和关系}
记得利用AI修改括号的形式
1.由
\begin{equation}
    \begin{aligned}
        \left( p\cdot \bar{\sigma} \right) \xi _{\lambda}\left( \mathbf{p} \right) &=\omega _{\lambda}^{2}\left( \mathbf{p} \right) \xi _{\lambda}\left( \mathbf{p} \right) 
\\
\left( p\cdot \sigma \right) \xi _{\lambda}\left( \mathbf{p} \right) &=\omega _{-\lambda}^{2}\left( \mathbf{p} \right) \xi _{\lambda}\left( \mathbf{p} \right) 
    \end{aligned}
\end{equation}
写出
\begin{equation}
    \begin{aligned}
        \left( p\cdot \bar{\sigma} \right) \xi _{-\lambda}\left( \mathbf{p} \right) &=\omega _{-\lambda}^{2}\left( \mathbf{p} \right) \xi _{-\lambda}\left( \mathbf{p} \right) 
\\
\left( p\cdot \sigma \right) \xi _{-\lambda}\left( \mathbf{p} \right) &=\omega _{\lambda}^{2}\left( \mathbf{p} \right) \xi _{-\lambda}\left( \mathbf{p} \right) 
    \end{aligned}
\end{equation}
2.由
\begin{equation}
    \sum_{\lambda =\pm}{\xi _{\lambda}}\left( \mathbf{p} \right) \xi _{\lambda}^{\dagger}\left( \mathbf{p} \right) =1
\end{equation}
写出
\begin{equation}
    \sum_{\lambda =\pm}{\xi _{-\lambda}}\left( \mathbf{p} \right) \xi _{-\lambda}^{\dagger}\left( \mathbf{p} \right) =1
\end{equation}
2.计算
\begin{equation}
    \begin{aligned}
        \sum_{\lambda =\pm}{u}\left( \mathbf{p},\lambda \right) \bar{u}\left( \mathbf{p},\lambda \right) &=\sum_{\lambda =\pm}{\left( \begin{array}{c}
	\omega _{-\lambda}\left( \mathbf{p} \right) \xi _{\lambda}\left( \mathbf{p} \right)\\
	\omega _{\lambda}\left( \mathbf{p} \right) \xi _{\lambda}\left( \mathbf{p} \right)\\
\end{array} \right)}\left( \begin{matrix}
	\omega _{\lambda}\left( \mathbf{p} \right) \xi _{\lambda}^{\dagger}\left( \mathbf{p} \right)&		\omega _{-\lambda}\left( \mathbf{p} \right) \xi _{\lambda}^{\dagger}\left( \mathbf{p} \right)\\
\end{matrix} \right) 
\\
&=\sum_{\lambda =\pm}{\left( \begin{matrix}
	\omega _{-\lambda}\left( \mathbf{p} \right) \omega _{\lambda}\left( \mathbf{p} \right) \xi _{\lambda}\left( \mathbf{p} \right) \xi _{\lambda}^{\dagger}\left( \mathbf{p} \right)&		\omega _{-\lambda}^{2}\left( \mathbf{p} \right) \xi _{\lambda}\left( \mathbf{p} \right) \xi _{\lambda}^{\dagger}\left( \mathbf{p} \right)\\
	\omega _{\lambda}^{2}\left( \mathbf{p} \right) \xi _{\lambda}\left( \mathbf{p} \right) \xi _{\lambda}^{\dagger}\left( \mathbf{p} \right)&		\omega _{\lambda}\left( \mathbf{p} \right) \omega _{-\lambda}\left( \mathbf{p} \right) \xi _{\lambda}\left( \mathbf{p} \right) \xi _{\lambda}^{\dagger}\left( \mathbf{p} \right)\\
\end{matrix} \right)}
\\
&=\sum_{\lambda =\pm}{\left( \begin{matrix}
	m\xi _{\lambda}\left( \mathbf{p} \right) \xi _{\lambda}^{\dagger}\left( \mathbf{p} \right)&		\left( p\cdot \sigma \right) \xi _{\lambda}\left( \mathbf{p} \right) \xi _{\lambda}^{\dagger}\left( \mathbf{p} \right)\\
	\left( p\cdot \bar{\sigma} \right) \xi _{\lambda}\left( \mathbf{p} \right) \xi _{\lambda}^{\dagger}\left( \mathbf{p} \right)&		m\xi _{\lambda}\left( \mathbf{p} \right) \xi _{\lambda}^{\dagger}\left( \mathbf{p} \right)\\
\end{matrix} \right)}
\\
&=\left( \begin{matrix}
	m&		p\cdot \sigma\\
	p\cdot \bar{\sigma}&		m\\
\end{matrix} \right) 
\\
&=\left( \begin{matrix}
	&		p\cdot \sigma\\
	p\cdot \bar{\sigma}&		\\
\end{matrix} \right) +\left( \begin{matrix}
	m&		\\
	&		m\\
\end{matrix} \right) 
\\
&=p_{\mu}\gamma ^{\mu}+m
    \end{aligned}
\end{equation}
同样地
\begin{equation}
    \begin{aligned}
        \sum_{\lambda =\pm}{v}\left( \mathbf{p},\lambda \right) \bar{v}\left( \mathbf{p},\lambda \right) &=\sum_{\lambda =\pm}{\left( \begin{array}{c}
	\lambda \omega _{\lambda}\left( \mathbf{p} \right) \xi _{-\lambda}\left( \mathbf{p} \right)\\
	-\lambda \omega _{-\lambda}\left( \mathbf{p} \right) \xi _{-\lambda}\left( \mathbf{p} \right)\\
\end{array} \right)}\left( \begin{matrix}
	-\lambda \omega _{-\lambda}\left( \mathbf{p} \right) \xi _{-\lambda}^{\dagger}\left( \mathbf{p} \right)&		\lambda \omega _{\lambda}\left( \mathbf{p} \right) \xi _{-\lambda}^{\dagger}\left( \mathbf{p} \right)\\
\end{matrix} \right) 
\\
&=\sum_{\lambda =\pm}{\left( \begin{matrix}
	-\lambda ^2\omega _{\lambda}\left( \mathbf{p} \right) \omega _{-\lambda}\left( \mathbf{p} \right) \xi _{-\lambda}\left( \mathbf{p} \right) \xi _{-\lambda}^{\dagger}\left( \mathbf{p} \right)&		\lambda ^2\omega _{\lambda}^{2}\left( \mathbf{p} \right) \xi _{-\lambda}\left( \mathbf{p} \right) \xi _{-\lambda}^{\dagger}\left( \mathbf{p} \right)\\
	\lambda ^2\omega _{-\lambda}^{2}\left( \mathbf{p} \right) \xi _{-\lambda}\left( \mathbf{p} \right) \xi _{-\lambda}^{\dagger}\left( \mathbf{p} \right)&		-\lambda ^2\omega _{-\lambda}\left( \mathbf{p} \right) \omega _{\lambda}\left( \mathbf{p} \right) \xi _{-\lambda}\left( \mathbf{p} \right) \xi _{-\lambda}^{\dagger}\left( \mathbf{p} \right)\\
\end{matrix} \right)}
\\
&=\sum_{\lambda =\pm}{\left( \begin{matrix}
	-m\xi _{-\lambda}\left( \mathbf{p} \right) \xi _{-\lambda}^{\dagger}\left( \mathbf{p} \right)&		\left( p\cdot \sigma \right) \xi _{-\lambda}\left( \mathbf{p} \right) \xi _{-\lambda}^{\dagger}\left( \mathbf{p} \right)\\
	\left( p\cdot \bar{\sigma} \right) \xi _{-\lambda}\left( \mathbf{p} \right) \xi _{-\lambda}^{\dagger}\left( \mathbf{p} \right)&		-m\xi _{-\lambda}\left( \mathbf{p} \right) \xi _{-\lambda}^{\dagger}\left( \mathbf{p} \right)\\
\end{matrix} \right)}
\\
&=\left( \begin{matrix}
	-m&		p\cdot \sigma\\
	p\cdot \bar{\sigma}&		-m\\
\end{matrix} \right) 
\\
&=\left( \begin{matrix}
	&		p\cdot \sigma\\
	p\cdot \bar{\sigma}&		\\
\end{matrix} \right) +\left( \begin{matrix}
	-m&		\\
	&		-m\\
\end{matrix} \right) 
\\
&=p_{\mu}\gamma ^{\mu}-m
    \end{aligned}
\end{equation}
其中
\begin{equation}
    \begin{aligned}
        \left( \begin{matrix}
	&		p\cdot \sigma\\
	p\cdot \bar{\sigma}&		\\
\end{matrix} \right) &=\left( \begin{matrix}
	&		p^0\sigma ^0-p^i\sigma ^i\\
	p^0\sigma ^0+p^i\sigma ^i&		\\
\end{matrix} \right) 
\\
&=\left( \begin{matrix}
	&		p^0\sigma ^0\\
	p^0\sigma ^0&		\\
\end{matrix} \right) +\left( \begin{matrix}
	&		-p^i\sigma ^i\\
	p^i\sigma ^i&		\\
\end{matrix} \right) 
\\
&=p^0\left( \begin{matrix}
	&		1\\
	1&		\\
\end{matrix} \right) -p^i\left( \begin{matrix}
	&		\sigma ^i\\
	-\sigma ^i&		\\
\end{matrix} \right) 
\\
&=p^0\gamma ^0-p^i\gamma ^i
\\
&=p_{\mu}\gamma ^{\mu}
    \end{aligned}
\end{equation}






